unusedglob/Callconv.v
@@ -1,0 +1,378 @@
+Require Export LogicalRelations.
+Require Export KLR.
+Require Export OptionRel.
+Require Export BoolRel.
+Require Export Valuesrel.
+
+Require Import Coqlib.
+Require Import Integers.
+Require Import AST.
+Require Import Values.
+Require Import Memory.
+Require Import Globalenvs.
+Require Import Events.
+Require Import LanguageInterface.
+
+Record cklr' :=
+  {
+    world: Type;
+    wacc: relation world;
+
+    cklr_kf : KripkeFrame unit world := {| acc w := wacc; |};
+
+    mi: world -> meminj;
+    match_mem: klr world mem mem;
+    match_stbls: klr world Genv.symtbl Genv.symtbl;
+
+    acc_preorder:
+      PreOrder wacc;
+
+    mi_acc:
+      Monotonic mi (wacc ++> inject_incr);
+    mi_acc_separated w w' m1 m2:
+      match_mem w m1 m2 ->
+      wacc w w' ->
+      inject_separated (mi w) (mi w') m1 m2;
+
+    match_stbls_acc:
+      Monotonic match_stbls (wacc ++> subrel);
+    match_stbls_proj w:
+      Related (match_stbls w) (Genv.match_stbls' (mi w)) subrel;
+    match_stbls_support w se1 se2 m1 m2:
+      match_stbls w se1 se2 ->
+      match_mem w m1 m2 ->
+      Mem.sup_include (Genv.genv_sup se1) (Mem.support m1) ->
+      Mem.sup_include (Genv.genv_sup se2) (Mem.support m2);
+
+    cklr_alloc:
+      Monotonic
+        (@Mem.alloc)
+        (|= match_mem ++> - ==> - ==>
+         <> match_mem * block_inject_sameofs @@ [mi]);
+
+    cklr_free:
+      Monotonic
+        (@Mem.free)
+        (|= match_mem ++> %% ptrrange_inject @@ [mi] ++>
+         k1 option_le (<> match_mem));
+
+    cklr_load:
+      Monotonic
+        (@Mem.load)
+        (|= - ==> match_mem ++> % ptr_inject @@ [mi] ++>
+         k1 option_le (Val.inject @@ [mi]));
+
+    cklr_store:
+      Monotonic
+        (@Mem.store)
+        (|= - ==> match_mem ++> % ptr_inject @@ [mi] ++> Val.inject @@ [mi] ++>
+         k1 option_le (<> match_mem));
+
+    cklr_loadbytes:
+      Monotonic
+        (@Mem.loadbytes)
+        (|= match_mem ++> % ptr_inject @@ [mi] ++> - ==>
+         k1 option_le (k1 list_rel (memval_inject @@ [mi])));
+
+    cklr_storebytes:
+      Monotonic
+        (@Mem.storebytes)
+        (|= match_mem ++> % rptr_inject @@ [mi] ++>
+         k1 list_rel (memval_inject @@ [mi]) ++>
+         k1 option_le (<> match_mem));
+
+    cklr_perm:
+      Monotonic
+        (@Mem.perm)
+        (|= match_mem ++> % ptr_inject @@ [mi] ++> - ==> - ==> k impl);
+
+    cklr_valid_block:
+      Monotonic
+        (@Mem.valid_block)
+        (|= match_mem ++> block_inject @@ [mi] ++> k iff);
+
+    cklr_no_overlap w m1 m2:
+      match_mem w m1 m2 ->
+      Mem.meminj_no_overlap (mi w) m1;
+
+    cklr_representable w m1 m2 b1 ofs1 b2 delta:
+      match_mem w m1 m2 ->
+      Mem.perm m1 b1 ofs1 Max Nonempty \/
+      Mem.perm m1 b1 (ofs1 - 1) Max Nonempty ->
+      mi w b1 = Some (b2, delta) ->
+      0 <= ofs1 <= Ptrofs.max_unsigned ->
+      delta >= 0 /\ 0 <= ofs1 + delta <= Ptrofs.max_unsigned;
+
+    (* similar to Mem.aligned_area_inject for memory injections.
+       Needed by Clight assign_of (By_copy) and memcpy. *)
+    cklr_aligned_area_inject:
+      forall w m m' b ofs al sz b' delta,
+        match_mem w m m' ->
+        (al = 1 \/ al = 2 \/ al = 4 \/ al = 8) ->
+        sz > 0 ->
+        (al | sz) ->
+        Mem.range_perm m b ofs (ofs + sz) Cur Nonempty ->
+        (al | ofs) ->
+        mi w b = Some (b', delta) ->
+        (al | ofs + delta);
+
+    (* similar to Mem.disjoint_or_equal_inject for memory injections.
+       Needed by Clight assign_of (By_copy) and memcpy. *)
+    cklr_disjoint_or_equal_inject:
+      forall w m m' b1 b1' delta1 b2 b2' delta2 ofs1 ofs2 sz,
+        match_mem w m m' ->
+        mi w b1 = Some (b1', delta1) ->
+        mi w b2 = Some (b2', delta2) ->
+        Mem.range_perm m b1 ofs1 (ofs1 + sz) Max Nonempty ->
+        Mem.range_perm m b2 ofs2 (ofs2 + sz) Max Nonempty ->
+        sz > 0 ->
+        b1 <> b2 \/
+        ofs1 = ofs2 \/
+        ofs1 + sz <= ofs2 \/ ofs2 + sz <= ofs1 ->
+        b1' <> b2' \/
+        (ofs1 + delta1 = ofs2 + delta2)%Z \/
+        ofs1 + delta1 + sz <= ofs2 + delta2 \/
+        ofs2 + delta2 + sz <= ofs1 + delta1;
+
+    cklr_perm_inv w m1 m2 b1 ofs1 b2 ofs2 k p:
+      match_mem w m1 m2 ->
+      ptr_inject (mi w) (b1, ofs1) (b2, ofs2) ->
+      Mem.perm m2 b2 ofs2 k p ->
+      Mem.perm m1 b1 ofs1 k p \/ ~Mem.perm m1 b1 ofs1 Max Nonempty;
+
+    cklr_sup_include w m1 m2 m1' m2':
+      match_mem w m1 m2 ->
+      (<> match_mem)%klr w m1' m2' ->
+      Mem.sup_include (Mem.support m1) (Mem.support m1') <->
+      Mem.sup_include (Mem.support m2) (Mem.support m2');
+
+  }.
+ 
+
+Record callconv' {li1 li2} :=
+  mk_callconv' {
+    ccworld' : Type;
+    match_senv': ccworld' -> Genv.symtbl -> Genv.symtbl -> Prop;
+    match_query': ccworld' -> query li1 -> query li2 -> Prop;
+    match_reply': ccworld' -> reply li1 -> reply li2 -> Prop;
+
+    match_senv_public_preserved':
+      forall w se1 se2,
+        match_senv' w se1 se2 ->
+        forall id, Genv.public_symbol se2 id = Genv.public_symbol se1 id;
+    (*match_senv_valid_for:
+      forall w se1 se2 sk,
+        match_senv w se1 se2 ->
+        Genv.valid_for sk se1 ->
+        Genv.valid_for sk se2; *)
+  }.
+
+Global Existing Instance cklr_kf.
+Global Existing Instance acc_preorder.
+Global Existing Instance mi_acc.
+Global Instance mi_acc_params: Params (@mi) 2 := {}.
+Global Existing Instance match_stbls_acc.
+Global Instance match_stbls_params: Params (@match_stbls) 3 := {}.
+
+Global Existing Instances cklr_alloc.
+Local Existing Instances cklr_free.
+Local Existing Instances cklr_load.
+Local Existing Instances cklr_store.
+Local Existing Instances cklr_loadbytes.
+Global Existing Instances cklr_storebytes.
+Local Existing Instances cklr_perm.
+Global Existing Instances cklr_valid_block.
+
+
+Arguments callconv': clear implicits.
+
+Inductive cc_c_query' R (w: world R): relation c_query :=
+  | cc_c_query_intro vf1 vf2 sg vargs1 vargs2 m1 m2:
+      Val.inject (mi R w) vf1 vf2 ->
+      Val.inject_list (mi R w) vargs1 vargs2 ->
+      match_mem R w m1 m2 ->
+      vf1 <> Vundef ->
+      cc_c_query' R w (cq vf1 sg vargs1 m1) (cq vf2 sg vargs2 m2).
+
+Inductive cc_c_reply' R (w: world R): relation c_reply :=
+  | cc_c_reply_intro vres1 vres2 m1' m2':
+      Val.inject (mi R w) vres1 vres2 ->
+      match_mem R w m1' m2' ->
+      cc_c_reply' R w (cr vres1 m1') (cr vres2 m2').
+
+Program Definition cc_c' (R: cklr'): callconv' li_c li_c :=
+  {|
+    ccworld' := world R;
+    match_senv' := match_stbls R;
+    match_query' := cc_c_query' R;
+    match_reply' := (<> cc_c_reply' R)%klr;
+  |}.
+Next Obligation.
+  intros. eapply match_stbls_proj in H. eapply Genv.mge_public'; eauto.
+Qed.
+
+Require Import Inject.
+
+Record inj_stbls' (w: inj_world) (se1 se2: Genv.symtbl): Prop :=
+  {
+    inj_stbls_match: Genv.match_stbls' (injw_meminj w) se1 se2;
+    inj_stbls_next_l: Mem.sup_include (Genv.genv_sup se1) (injw_sup_l w);
+    inj_stbls_next_r: Mem.sup_include (Genv.genv_sup se2) (injw_sup_r w);
+  }.
+
+Global Instance inj_stbls_subrel':
+  Monotonic inj_stbls' (inj_incr ++> subrel).
+Proof.
+  intros w w' Hw se1 se2 Hse.
+  destruct Hse; inv Hw. cbn in *.
+  constructor; cbn; try extlia.
+  eapply Genv.match_stbls_incr'; eauto.
+  intros. edestruct H0; eauto.
+  split; eauto. eauto. eauto.
+Qed.
+
+Program Definition inj' : cklr' :=
+  {|
+    world := inj_world;
+    wacc := inj_incr;
+    mi := injw_meminj;
+    match_stbls := inj_stbls';
+    match_mem := inj_mem;
+  |}.
+
+Next Obligation. (* mi_acc_separated *)
+  eapply inj_acc_separated; eauto.
+Qed.
+
+Next Obligation.
+  destruct 1. cbn. auto.
+Qed.
+
+Next Obligation.
+  destruct H. inv H0; cbn in *. eauto.
+Qed.
+
+Next Obligation. (* Mem.alloc *)
+  exact inj_cklr_alloc.
+Qed.
+
+
+Next Obligation. (* Mem.free *)
+  intros [f nb1 nb2] m1 m2 Hm [[b1 lo1] hi1] [[b2 lo2] hi2] Hr.
+  simpl. red.
+  destruct (Mem.free m1 b1 lo1 hi1) as [m1'|] eqn:Hm1'; [|rauto].
+  inv Hr. cbn in H0. inv H0. inv Hm.
+  edestruct Mem.free_parallel_inject as (m2' & Hm2' & Hm'); eauto.
+  replace (lo1 + delta + sz) with (lo1 + sz + delta) by extlia.
+  rewrite Hm2'.
+  repeat (econstructor; eauto); try congruence;
+    erewrite <- Mem.support_free; eauto.
+Qed.
+
+Next Obligation. (* Mem.load *)
+  intros [f nb1 nb2] chunk m1 m2 Hm _ _ [b1 ofs1 b2 delta Hptr].
+  cbn in *. red. inv Hm.
+  destruct (Mem.load chunk m1 b1 ofs1) as [v1|] eqn:Hv1; [|rauto].
+  edestruct Mem.load_inject as (v2 & Hv2 & Hv); eauto.
+  rewrite Hv2. repeat (econstructor; eauto).
+Qed.
+
+Next Obligation. (* Mem.store *)
+  intros [f nb1 nb2] chunk m1 m2 Hm _ _ [b1 ofs1 b2 delta Hptr] v1 v2 Hv.
+  red in Hv |- *. cbn in *. inv Hm.
+  destruct (Mem.store chunk m1 b1 ofs1 v1) as [m1'|] eqn:Hm1'; [|rauto].
+  edestruct Mem.store_mapped_inject as (m2' & Hm2' & Hm'); eauto.
+  rewrite Hm2'.
+  repeat (econstructor; eauto); try congruence;
+    erewrite <- Mem.support_store; eauto.
+Qed.
+
+Next Obligation. (* Mem.loadbytes *)
+  intros [f nb1 nb2] m1 m2 Hm _ _ [b1 ofs1 b2 delta Hptr] sz.
+  red. cbn in *. inv Hm.
+  destruct (Mem.loadbytes m1 b1 ofs1 sz) as [vs1|] eqn:Hvs1; [|rauto].
+  edestruct Mem.loadbytes_inject as (vs2 & Hvs2 & Hvs); eauto.
+  rewrite Hvs2. rauto.
+Qed.
+
+Next Obligation. (* Mem.storebytes *)
+  intros [f nb1 nb2] m1 m2 Hm [b1 ofs1] [b2 ofs2] Hptr vs1 vs2 Hvs.
+  red in Hvs |- *. cbn in *. inv Hm.
+  destruct (Mem.storebytes m1 _ _ _) as [m1'|] eqn:Hm1'; [|constructor].
+  assert (vs1 = nil \/ vs1 <> nil) as [Hvs1|Hvs1].
+  { destruct vs1; constructor; congruence. }
+  - subst. inv Hvs.
+    edestruct (Mem.range_perm_storebytes m2 b2 ofs2 nil) as [m2' Hm2'].
+    {
+      intros ofs. simpl. extlia.
+    }
+    rewrite Hm2'.
+    constructor.
+    eexists; split; repeat rstep.
+    erewrite <- (Mem.support_storebytes m1); eauto.
+    erewrite <- (Mem.support_storebytes m2); eauto.
+    constructor; eauto.
+    eapply Mem.storebytes_empty_inject; eauto.
+  - assert (ptr_inject f (b1, ofs1) (b2, ofs2)) as Hptr'.
+    {
+      destruct Hptr as [Hptr|Hptr]; eauto.
+      inversion Hptr as [_ _ [xb1 xofs1 xb2 delta Hb]]; clear Hptr; subst.
+      unfold ptrbits_unsigned.
+      erewrite Mem.address_inject; eauto.
+      apply Mem.storebytes_range_perm in Hm1'.
+      eapply Hm1'.
+      destruct vs1; try congruence.
+      simpl. extlia.
+    }
+    inv Hptr'.
+    edestruct Mem.storebytes_mapped_inject as (m2' & Hm2' & Hm'); eauto. rauto.
+    rewrite Hm2'.
+    repeat (econstructor; eauto); try congruence;
+      erewrite <- Mem.support_storebytes; eauto.
+Qed.
+
+Next Obligation. (* Mem.perm *)
+  intros [f nb1 nb2] m1 m2 Hm _ _ [b1 ofs1 b2 delta Hb] p k H.
+  eapply Mem.perm_inject; eauto.
+Qed.
+
+Next Obligation. (* Mem.valid_block *)
+  intros [f nb1 nb2] m1 m2 Hm b1 b2 [delta Hb].
+  split; intro.
+  - eapply Mem.valid_block_inject_2; eauto.
+  - eapply Mem.valid_block_inject_1; eauto.
+Qed.
+
+Next Obligation. (* Mem.meminj_no_overlap *)
+  destruct H as [f m1 m2 nb1].
+  eapply Mem.mi_no_overlap; eauto.
+Qed.
+
+Next Obligation. (* representable *)
+  destruct H as [f m1 m2 nb1].
+  rewrite <- (Ptrofs.unsigned_repr ofs1) by extlia.
+  eapply Mem.mi_representable; eauto.
+  rewrite Ptrofs.unsigned_repr by extlia.
+  assumption.
+Qed.
+
+Next Obligation.
+  destruct H.
+  eapply Mem.aligned_area_inject; eauto.
+Qed.
+
+Next Obligation. 
+  destruct H.
+  eapply Mem.disjoint_or_equal_inject; eauto.
+Qed.
+
+Next Obligation. (* perm_inv *)
+  destruct H. inv H0.
+  eapply Mem.perm_inject_inv; eauto.
+Qed.
+
+Next Obligation. (* nextblock incr *)
+  destruct H0 as (w' & Hw' & Hm').
+  destruct H. inv Hm'. inv Hw'.
+  split; auto.
+Qed.
