unusedglob/ForwardSim.v
@@ -1,0 +1,323 @@
+Require Import Relations.
+Require Import Wellfounded.
+Require Import Coqlib.
+Require Import Events.
+Require Import Globalenvs.
+Require Import LanguageInterface.
+Require Import Integers.
+Require Import Smallstep.
+Require Import Callconv.
+
+Set Implicit Arguments.
+
+Section FSIM'.
+
+Context {liA1 liA2} (ccA: callconv' liA1 liA2).
+Context {liB1 liB2} (ccB: callconv' liB1 liB2).
+Context (se1 se2: Genv.symtbl) (wB: ccworld' ccB).
+Context {state1 state2: Type}.
+
+(** The general form of a forward simulation. *)
+
+Record fsim_properties' (L1: lts liA1 liB1 state1) (L2: lts liA2 liB2 state2) (index: Type)
+                       (order: index -> index -> Prop)
+                       (match_states: index -> state1 -> state2 -> Prop) : Prop := {
+    fsim_match_valid_query':
+      forall q1 q2, match_query' ccB wB q1 q2 ->
+      valid_query L2 q2 = valid_query L1 q1;
+    fsim_match_initial_states':
+      forall q1 q2 s1, match_query' ccB wB q1 q2 -> initial_state L1 q1 s1 ->
+      exists i, exists s2, initial_state L2 q2 s2 /\ match_states i s1 s2;
+    fsim_match_final_states':
+      forall i s1 s2 r1, match_states i s1 s2 -> final_state L1 s1 r1 ->
+      exists r2, final_state L2 s2 r2 /\ match_reply' ccB wB r1 r2;
+    fsim_match_external':
+      forall i s1 s2 q1, match_states i s1 s2 -> at_external L1 s1 q1 ->
+      exists w q2, at_external L2 s2 q2 /\ match_query' ccA w q1 q2 /\ match_senv' ccA w se1 se2 /\
+      forall r1 r2 s1', match_reply' ccA w r1 r2 -> after_external L1 s1 r1 s1' ->
+      exists i' s2', after_external L2 s2 r2 s2' /\ match_states i' s1' s2';
+    fsim_simulation_1:
+      forall s1 t s1', Step L1 s1 t s1' ->
+      forall i s2, match_states i s1 s2 ->
+      exists i', exists s2',
+         (Plus L2 s2 t s2' \/ (Star L2 s2 t s2' /\ order i' i))
+      /\ match_states i' s1' s2';
+  }.
+
+Arguments fsim_properties' : clear implicits.
+
+(** An alternate form of the simulation diagram *)
+
+Lemma fsim_simulation'_1:
+  forall L1 L2 index order match_states, fsim_properties' L1 L2 index order match_states ->
+  forall i s1 t s1', Step L1 s1 t s1' ->
+  forall s2, match_states i s1 s2 ->
+  (exists i', exists s2', Plus L2 s2 t s2' /\ match_states i' s1' s2')
+  \/ (exists i', order i' i /\ t = E0 /\ match_states i' s1' s2).
+Proof.
+  intros. exploit @fsim_simulation_1; eauto.
+  intros [i' [s2' [A B]]]. intuition.
+  left; exists i'; exists s2'; auto.
+  inv H3.
+  right; exists i'; auto.
+  left; exists i'; exists s2'; split; auto. econstructor; eauto.
+Qed.
+
+(** ** Forward simulation diagrams. *)
+
+(** Various simulation diagrams that imply forward simulation *)
+
+Section FORWARD_SIMU_DIAGRAMS.
+
+Variable L1: lts liA1 liB1 state1.
+Variable L2: lts liA2 liB2 state2.
+
+Variable match_states: state1 -> state2 -> Prop.
+
+Hypothesis match_valid_query:
+  forall q1 q2, match_query' ccB wB q1 q2 ->
+  valid_query L2 q2 = valid_query L1 q1.
+
+Hypothesis match_initial_states:
+  forall q1 q2 s1, match_query' ccB wB q1 q2 -> initial_state L1 q1 s1 ->
+  exists s2, initial_state L2 q2 s2 /\ match_states s1 s2.
+
+Hypothesis match_final_states:
+  forall s1 s2 r1, match_states s1 s2 -> final_state L1 s1 r1 ->
+  exists r2, final_state L2 s2 r2 /\ match_reply' ccB wB r1 r2.
+
+Hypothesis match_external:
+  forall s1 s2 q1, match_states s1 s2 -> at_external L1 s1 q1 ->
+  exists wA q2, at_external L2 s2 q2 /\ match_query' ccA wA q1 q2 /\ match_senv' ccA wA se1 se2 /\
+  forall r1 r2 s1', match_reply' ccA wA r1 r2 -> after_external L1 s1 r1 s1' ->
+  exists s2', after_external L2 s2 r2 s2' /\ match_states s1' s2'.
+
+Let ms idx s1 s2 := idx = s1 /\ match_states s1 s2.
+
+(** Simulation when one transition in the first program
+    corresponds to zero, one or several transitions in the second program.
+    However, there is no stuttering: infinitely many transitions
+    in the source program must correspond to infinitely many
+    transitions in the second program. *)
+
+Section SIMULATION_STAR_WF.
+
+(** [order] is a well-founded ordering associated with states
+  of the first semantics.  Stuttering steps must correspond
+  to states that decrease w.r.t. [order]. *)
+
+Variable order: state1 -> state1 -> Prop.
+
+Hypothesis simulation:
+  forall s1 t s1', Step L1 s1 t s1' ->
+  forall s2, match_states s1 s2 ->
+  exists s2',
+  (Plus L2 s2 t s2' \/ (Star L2 s2 t s2' /\ order s1' s1))
+  /\ match_states s1' s2'.
+
+Lemma forward_simulation_star_wf':
+  fsim_properties' L1 L2 state1 order ms.
+Proof.
+  subst ms;
+  constructor.
+- auto.
+- intros. exploit match_initial_states; eauto. intros [s2 [A B]].
+    exists s1; exists s2; auto.
+- intros. destruct H. eapply match_final_states; eauto.
+- intros. destruct H. edestruct match_external as (w & q2 & H2 & Hq & Hw & Hr); eauto.
+  exists w, q2. intuition auto. edestruct Hr as (s2' & Hs2' & Hs'); eauto.
+- intros. destruct H0. subst i. exploit simulation; eauto. intros [s2' [A B]].
+  exists s1'; exists s2'; intuition auto.
+Qed.
+
+End SIMULATION_STAR_WF.
+
+Section SIMULATION_STAR.
+
+(** We now consider the case where we have a nonnegative integer measure
+  associated with states of the first semantics.  It must decrease when we take
+  a stuttering step. *)
+
+Variable measure: state1 -> nat.
+
+Hypothesis simulation:
+  forall s1 t s1', Step L1 s1 t s1' ->
+  forall s2, match_states s1 s2 ->
+  (exists s2', Plus L2 s2 t s2' /\ match_states s1' s2')
+  \/ (measure s1' < measure s1 /\ t = E0 /\ match_states s1' s2)%nat.
+
+Lemma forward_simulation_star':
+  fsim_properties' L1 L2 state1 (ltof _ measure) ms.
+Proof.
+  apply forward_simulation_star_wf'.
+  intros. exploit simulation; eauto. intros [[s2' [A B]] | [A [B C]]].
+  exists s2'; auto.
+  exists s2; split. right; split. rewrite B. apply star_refl. auto. auto.
+Qed.
+
+End SIMULATION_STAR.
+
+(** Simulation when one transition in the first program corresponds
+    to one or several transitions in the second program. *)
+
+Section SIMULATION_PLUS.
+
+Hypothesis simulation:
+  forall s1 t s1', Step L1 s1 t s1' ->
+  forall s2, match_states s1 s2 ->
+  exists s2', Plus L2 s2 t s2' /\ match_states s1' s2'.
+
+Lemma forward_simulation_plus':
+  fsim_properties' L1 L2 state1 (ltof _ (fun _ => O)) ms.
+Proof.
+  apply forward_simulation_star'.
+  intros. exploit simulation; eauto.
+Qed.
+
+End SIMULATION_PLUS.
+
+(** Lock-step simulation: each transition in the first semantics
+    corresponds to exactly one transition in the second semantics. *)
+
+Section SIMULATION_STEP.
+
+Hypothesis simulation:
+  forall s1 t s1', Step L1 s1 t s1' ->
+  forall s2, match_states s1 s2 ->
+  exists s2', Step L2 s2 t s2' /\ match_states s1' s2'.
+
+Lemma forward_simulation_step':
+  fsim_properties' L1 L2 state1 (ltof _ (fun _ => O)) ms.
+Proof.
+  apply forward_simulation_plus'.
+  intros. exploit simulation; eauto. intros [s2' [A B]].
+  exists s2'; split; auto. apply plus_one; auto.
+Qed.
+
+End SIMULATION_STEP.
+
+(** Simulation when one transition in the first program
+    corresponds to zero or one transitions in the second program.
+    However, there is no stuttering: infinitely many transitions
+    in the source program must correspond to infinitely many
+    transitions in the second program. *)
+
+Section SIMULATION_OPT.
+
+Variable measure: state1 -> nat.
+
+Hypothesis simulation:
+  forall s1 t s1', Step L1 s1 t s1' ->
+  forall s2, match_states s1 s2 ->
+  (exists s2', Step L2 s2 t s2' /\ match_states s1' s2')
+  \/ (measure s1' < measure s1 /\ t = E0 /\ match_states s1' s2)%nat.
+
+Lemma forward_simulation_opt':
+  fsim_properties' L1 L2 state1 (ltof _ measure) ms.
+Proof.
+  apply forward_simulation_star'.
+  intros. exploit simulation; eauto. intros [[s2' [A B]] | [A [B C]]].
+  left; exists s2'; split; auto. apply plus_one; auto.
+  right; auto.
+Qed.
+
+End SIMULATION_OPT.
+
+End FORWARD_SIMU_DIAGRAMS.
+
+(** ** Forward simulation of transition sequences *)
+
+Section SIMULATION_SEQUENCES.
+
+Context L1 L2 index order match_states (S: fsim_properties' L1 L2 index order match_states).
+
+Lemma simulation_star':
+  forall s1 t s1', Star L1 s1 t s1' ->
+  forall i s2, match_states i s1 s2 ->
+  exists i', exists s2', Star L2 s2 t s2' /\ match_states i' s1' s2'.
+Proof.
+  induction 1; intros.
+  exists i; exists s2; split; auto. apply star_refl.
+  exploit fsim_simulation_1; eauto. intros [i' [s2' [A B]]].
+  exploit IHstar; eauto. intros [i'' [s2'' [C D]]].
+  exists i''; exists s2''; split; auto. eapply star_trans; eauto.
+  intuition auto. apply plus_star; auto.
+Qed.
+
+Lemma simulation_plus':
+  forall s1 t s1', Plus L1 s1 t s1' ->
+  forall i s2, match_states i s1 s2 ->
+  (exists i', exists s2', Plus L2 s2 t s2' /\ match_states i' s1' s2')
+  \/ (exists i', clos_trans _ order i' i /\ t = E0 /\ match_states i' s1' s2).
+Proof.
+  induction 1 using plus_ind2; intros.
+(* base case *)
+  exploit fsim_simulation'_1; eauto. intros [A | [i' A]].
+  left; auto.
+  right; exists i'; intuition.
+(* inductive case *)
+  exploit fsim_simulation'_1; eauto. intros [[i' [s2' [A B]]] | [i' [A [B C]]]].
+  exploit simulation_star'. apply plus_star; eauto. eauto.
+  intros [i'' [s2'' [P Q]]].
+  left; exists i''; exists s2''; split; auto. eapply plus_star_trans; eauto.
+  exploit IHplus; eauto. intros [[i'' [s2'' [P Q]]] | [i'' [P [Q R]]]].
+  subst. simpl. left; exists i''; exists s2''; auto.
+  subst. simpl. right; exists i''; intuition auto.
+  eapply t_trans; eauto. eapply t_step; eauto.
+Qed.
+
+Lemma simulation_forever_silent':
+  well_founded order ->
+  forall i s1 s2,
+  Forever_silent L1 s1 -> match_states i s1 s2 ->
+  Forever_silent L2 s2.
+Proof.
+  assert (forall i s1 s2,
+          Forever_silent L1 s1 -> match_states i s1 s2 ->
+          forever_silent_N (step L2) order (globalenv L2) i s2).
+    cofix COINDHYP; intros.
+    inv H. destruct (fsim_simulation_1 S _ _ _ H1 _ _ H0) as [i' [s2' [A B]]].
+    destruct A as [C | [C D]].
+    eapply forever_silent_N_plus; eauto.
+    eapply forever_silent_N_star; eauto.
+  intros. eapply forever_silent_N_forever; eauto.
+Qed.
+
+Lemma simulation_forever_reactive':
+  forall i s1 s2 T,
+  Forever_reactive L1 s1 T -> match_states i s1 s2 ->
+  Forever_reactive L2 s2 T.
+Proof.
+  cofix COINDHYP; intros.
+  inv H.
+  edestruct simulation_star' as [i' [st2' [A B]]]; eauto.
+  econstructor; eauto.
+Qed.
+
+End SIMULATION_SEQUENCES.
+
+End FSIM'.
+
+Arguments fsim_properties' {_ _} _ {_ _} _ _ _ _ {_ _} L1 L2 index order match_states.
+
+Record fsim_components' {liA1 liA2} (ccA: callconv' liA1 liA2) {liB1 liB2} ccB L1 L2 :=
+  Forward_simulation' {
+    fsim_index': Type;
+    fsim_order': fsim_index' -> fsim_index' -> Prop;
+    fsim_match_states': _;
+
+    fsim_skel':
+      Genv.skel_le (skel L2) (skel L1);
+    fsim_lts' se1 se2 wB:
+      @match_senv' liB1 liB2 ccB wB se1 se2 ->
+      Genv.skel_symtbl_compatible (skel L1) (skel L2) se1 se2 ->
+      fsim_properties' ccA ccB se1 se2 wB (activate L1 se1) (activate L2 se2)
+        fsim_index' fsim_order' (fsim_match_states' se1 se2 wB);
+    fsim_order_wf':
+      well_founded fsim_order';
+  }.
+
+Arguments Forward_simulation' {_ _ ccA _ _ ccB L1 L2 fsim_index'}.
+
+Definition forward_simulation' {liA1 liA2} ccA {liB1 liB2} ccB L1 L2 :=
+  inhabited (@fsim_components' liA1 liA2 ccA liB1 liB2 ccB L1 L2).
